theories/lang_oadt/semantics.v
@@ -7,6 +7,32 @@ Import syntax.notations.
 
 Implicit Types (b : bool).
 
+(** ** Weak values *)
+Inductive wval : expr -> Prop :=
+| WUnitV : wval <{ () }>
+| WLit b : wval <{ lit b }>
+| WPair v1 v2 : wval v1 -> wval v2 -> wval <{ (v1, v2) }>
+| WAbs l τ e : wval <{ \:{l}τ => e }>
+| WInj b τ v : wval v -> wval <{ inj@b<τ> v }>
+| WFold X v : wval v -> wval <{ fold<X> v }>
+| WBoxedLit b : wval <{ [b] }>
+| WBoxedInj b ω v : otval ω -> oval v -> wval <{ [inj@b<ω> v] }>
+| WIte v0 v1 v2 :
+    wval v0 -> wval v1 -> wval v2 ->
+    wval <{ ~if v0 then v1 else v2 }>
+.
+
+(** ** Weak oblivious values *)
+Inductive woval : expr -> Prop :=
+| OWUnitV : woval <{ () }>
+| OWBoxedLit b : woval <{ [b] }>
+| OWPair v1 v2 : woval v1 -> woval v2 -> woval <{ (v1, v2) }>
+| OWBoxedInj b ω v : otval ω -> oval v -> woval <{ [inj@b<ω> v] }>
+| OWIte v0 v1 v2 :
+    woval v0 -> woval v1 -> woval v2 ->
+    woval <{ ~if v0 then v1 else v2 }>
+.
+
 (** ** OADT value typing *)
 (** [ovalty v ω] means [v] is an oblivious value of oblivious type value [ω].
 This is essentially a subset of [typing], but we have it so that the dynamic
@@ -29,30 +55,42 @@ Inductive ovalty : expr -> expr -> Prop :=
 (** We define evaluation context [ℇ] as the hole-filling function. [ℇ e] fills
 the hole in [ℇ] with [e]. [ectx ℇ] asserts that [ℇ] is a well-formed
 context. *)
-Inductive ectx : (expr -> expr) -> Prop :=
-(* | CtxTop : ectx (fun e => e) *)
+
+(** Note that we reduce applications from right to left for some subtle reason. *)
+
+(** The evaluation context enclosing possibly leaking expressions. *)
+Variant lectx : (expr -> expr) -> Prop :=
+| CtxApp1 v2 : wval v2 -> lectx (fun e1 => <{ e1 v2 }>)
+| CtxSec : lectx (fun e => <{ s𝔹 e }>)
+| CtxIte e1 e2 : lectx (fun e0 => <{ if e0 then e1 else e2 }>)
+| CtxProj b : lectx (fun e => <{ π@b e }>)
+| CtxCase e1 e2: lectx (fun e0 => <{ case e0 of e1 | e2 }>)
+| CtxUnfold X : lectx (fun e => <{ unfold<X> e }>)
+.
+
+(** The top-level evaluation context. *)
+Variant ectx : (expr -> expr) -> Prop :=
 | CtxProd1 τ2 : ectx (fun τ1 => <{ τ1 * τ2 }>)
 | CtxProd2 ω1 : otval ω1 -> ectx (fun τ2 => <{ ω1 * τ2 }>)
 | CtxOSum1 τ2 : ectx (fun τ1 => <{ τ1 ~+ τ2 }>)
 | CtxOSum2 ω1 : otval ω1 -> ectx (fun τ2 => <{ ω1 ~+ τ2 }>)
-(** We reduce applications from right to left for some subtle reason. *)
-| CtxApp1 e1 : ectx (fun e2 => <{ e1 e2 }>)
-| CtxApp2 v2 : val v2 -> ectx (fun e1 => <{ e1 v2 }>)
+| CtxApp2 e1 : ectx (fun e2 => <{ e1 e2 }>)
 | CtxLet e2 : ectx (fun e1 => <{ let e1 in e2 }>)
-| CtxSec : ectx (fun e => <{ s𝔹 e }>)
-| CtxIte e1 e2 : ectx (fun e0 => <{ if e0 then e1 else e2 }>)
-| CtxMux1 e1 e2 : ectx (fun e0 => <{ ~if e0 then e1 else e2 }>)
-| CtxMux2 v0 e2 : val v0 -> ectx (fun e1 => <{ ~if v0 then e1 else e2 }>)
-| CtxMux3 v0 v1 : val v0 -> val v1 -> ectx (fun e2 => <{ ~if v0 then v1 else e2 }>)
+| CtxOIte1 e1 e2 : ectx (fun e0 => <{ ~if e0 then e1 else e2 }>)
+| CtxOIte2 v0 e2 : wval v0 -> ectx (fun e1 => <{ ~if v0 then e1 else e2 }>)
+| CtxOIte3 v0 v1 : wval v0 -> wval v1 -> ectx (fun e2 => <{ ~if v0 then v1 else e2 }>)
+| CtxOCase e1 e2: ectx (fun e0 => <{ ~case e0 of e1 | e2 }>)
 | CtxPair1 e2 : ectx (fun e1 => <{ (e1, e2) }>)
-| CtxPair2 v1 : val v1 -> ectx (fun e2 => <{ (v1, e2) }>)
-| CtxProj b : ectx (fun e => <{ π@b e }>)
+| CtxPair2 v1 : wval v1 -> ectx (fun e2 => <{ (v1, e2) }>)
 | CtxInj b τ : ectx (fun e => <{ inj@b<τ> e }>)
 | CtxOInj1 b e : ectx (fun τ => <{ ~inj@b<τ> e }>)
 | CtxOInj2 b ω : otval ω -> ectx (fun e => <{ ~inj@b<ω> e }>)
-| CtxCase l e1 e2: ectx (fun e0 => <{ case{l} e0 of e1 | e2 }>)
 | CtxFold X : ectx (fun e => <{ fold<X> e }>)
-| CtxUnfold X : ectx (fun e => <{ unfold<X> e }>)
+| CtxTape : ectx (fun e => <{ tape e }>)
+| CtxMux1 e1 e2 : ectx (fun e0 => <{ mux e0 e1 e2 }>)
+| CtxMux2 v0 e2 : wval v0 -> ectx (fun e1 => <{ mux v0 e1 e2 }>)
+| CtxMux3 v0 v1 : wval v0 -> wval v1 -> ectx (fun e2 => <{ mux v0 v1 e2 }>)
+| CtxLeak ℇ : lectx ℇ -> ectx ℇ
 .
 
 (** ** Small-step relation *)
@@ -61,46 +99,63 @@ Section step.
 Reserved Notation "e '-->!' e'" (at level 40).
 
 Inductive step (Σ : gctx) : expr -> expr -> Prop :=
-| SApp τ e v :
-    val v ->
-    <{ (\:τ => e) v }> -->! <{ e^v }>
+| SApp l τ e v :
+    wval v ->
+    <{ (\:{l}τ => e) v }> -->! <{ e^v }>
 | SLet v e :
-    val v ->
+    wval v ->
     <{ let v in e }> -->! <{ e^v }>
 | SCase b τ v e1 e2 :
-    val v ->
+    wval v ->
     <{ case inj@b<τ> v of e1 | e2 }> -->! <{ ite b (e1^v) (e2^v) }>
-(** The most interesting rule *)
+(** One of the most interesting rules. *)
 | SOCase b ω1 ω2 v e1 e2 v1 v2 :
     oval v ->
     ovalty v1 ω1 -> ovalty v2 ω2 ->
     <{ ~case [inj@b<ω1 ~+ ω2> v] of e1 | e2 }> -->!
       <{ ~if [b] then (ite b (e1^v) (e1^v1)) else (ite b (e2^v2) (e2^v)) }>
 | SAppOADT X τ e v :
-    val v ->
+    wval v ->
     Σ !! X = Some (DOADT τ e) ->
     <{ (gvar X) v }> -->! <{ e^v }>
-| SAppFun x τ e :
-    Σ !! x = Some (DFun τ e) ->
+| SAppFun x T e :
+    Σ !! x = Some (DFun T e) ->
     <{ gvar x }> -->! <{ e }>
 | SOInj b ω v :
     otval ω -> oval v ->
     <{ ~inj@b<ω> v }> -->! <{ [inj@b<ω> v] }>
 | SIte b e1 e2 :
     <{ if b then e1 else e2 }> -->! <{ ite b e1 e2 }>
-(** If we also want runtime obliviousness (e.g., against malicious adversaries),
-we can check [v1] and [v2] are oblivious values in this rule. *)
-| SMux b v1 v2 :
-    val v1 -> val v2 ->
-    <{ ~if [b] then v1 else v2 }> -->! <{ ite b v1 v2 }>
 | SProj b v1 v2 :
-    val v1 -> val v2 ->
+    wval v1 -> wval v2 ->
     <{ π@b (v1, v2) }> -->! <{ ite b v1 v2 }>
 | SFold X X' v :
-    val v ->
+    wval v ->
     <{ unfold<X> (fold <X'> v) }> -->! v
 | SSec b :
     <{ s𝔹 b }> -->! <{ [b] }>
+| SMux b v1 v2 :
+    wval v1 -> wval v2 ->
+    <{ mux [b] v1 v2 }> -->! <{ ite b v1 v2 }>
+| STapeOIte b v1 v2 :
+    woval v1 -> woval v2 ->
+    <{ tape (~if [b] then v1 else v2) }> -->! <{ mux [b] (tape v1) (tape v2) }>
+| STapePair v1 v2 :
+    woval v1 -> woval v2 ->
+    <{ tape (v1, v2) }> -->! <{ (tape v1, tape v2) }>
+(** [tape v] is a no-op if [v] is an oblivious value (except for pair). Spell
+out all the cases here for determinism and proof convenience. *)
+| STapeUnitV :
+    <{ tape () }> -->! <{ () }>
+| STapeBoxedLit b :
+    <{ tape [b] }> -->! <{ [b] }>
+| STapeBoxedInj b ω v :
+    otval ω -> oval v ->
+    <{ tape [inj@b<ω> v] }> -->! <{ [inj@b<ω> v] }>
+| SOIte b v1 v2 ℇ :
+    lectx ℇ ->
+    wval v1 -> wval v2 ->
+    ℇ <{ ~if [b] then v1 else v2 }> -->! <{ ~if [b] then ,(ℇ v1) else ,(ℇ v2) }>
 (** Step under evaluation context *)
 | SCtx ℇ e e' :
     ectx ℇ ->
