theories/lang_oadt/typing.v
@@ -20,6 +20,7 @@ Variant kind :=
 
 (** [kind] has (semi-)lattice operators. *)
 
+
 (** We define the partial order [⊑] on [kind] directly as a computable
 function. Alternatively, we may define an "immediate" relation as the kernel,
 and then take its reflexive-transitive closure. But [kind] is simple enough, so
@@ -56,7 +57,7 @@ Instance kind_top : Top kind := KMixed.
 Instance kind_bot : Bottom kind := KAny.
 
 (** ** Typing context (Γ) *)
-Notation tctx := (amap expr).
+Notation tctx := (amap lexpr).
 
 (** Notations for kinding *)
 Module kind_notations.
@@ -88,11 +89,11 @@ Reserved Notation "e '==>!' e'" (at level 40,
                                  e' constr at level 0).
 
 Inductive pared : expr -> expr -> Prop :=
-| RApp τ e1 e2 e1' e2' L :
+| RApp l τ e1 e2 e1' e2' L :
     e1 ==>! e1' ->
     (forall x, x ∉ L -> <{ e2^x }> ==>! <{ e2'^x }>) ->
     lc τ ->
-    <{ (\:τ => e2) e1 }> ==>! <{ e2'^e1' }>
+    <{ (\:{l}τ => e2) e1 }> ==>! <{ e2'^e1' }>
 | RLet e1 e2 e1' e2' L :
     e1 ==>! e1' ->
     (forall x, x ∉ L -> <{ e2^x }> ==>! <{ e2'^x }>) ->
@@ -101,8 +102,8 @@ Inductive pared : expr -> expr -> Prop :=
     Σ !! X = Some (DOADT τ e2) ->
     e1 ==>! e1' ->
     <{ (gvar X) e1 }> ==>! <{ e2^e1' }>
-| RAppFun x τ e :
-    Σ !! x = Some (DFun τ e) ->
+| RAppFun x T e :
+    Σ !! x = Some (DFun T e) ->
     <{ gvar x }> ==>! <{ e }>
 | RProj b e1 e2 e1' e2' :
     e1 ==>! e1' ->
@@ -126,6 +127,11 @@ not needed because they are not involved in type-level computation. *)
 | RMux b e1 e2 e1' e2' :
     e1 ==>! e1' ->
     e2 ==>! e2' ->
+    <{ mux [b] e1 e2 }> ==>! <{ ite b e1' e2' }>
+(* This rule is needed for confluence. *)
+| ROIte b e1 e2 e1' e2' :
+    e1 ==>! e1' ->
+    e2 ==>! e2' ->
     <{ ~if [b] then e1 else e2 }> ==>! <{ ite b e1' e2' }>
 | ROCase b ω1 ω2 v v1 v2 e1 e2 e1' e2' L1 L2 :
     oval v ->
@@ -139,6 +145,57 @@ not needed because they are not involved in type-level computation. *)
 | ROInj b ω v :
     otval ω -> oval v ->
     <{ ~inj@b<ω> v }> ==>! <{ [inj@b<ω> v] }>
+(* Unfortunately I have to spell out all the cases corresponding to [SOIte] for
+proof convenience. *)
+| ROIteApp b e1 e2 e e1' e2' e' :
+    e1 ==>! e1' ->
+    e2 ==>! e2' ->
+    e ==>! e' ->
+    <{ (~if [b] then e1 else e2) e }> ==>! <{ ~if [b] then e1' e' else e2' e' }>
+| ROIteSec b e1 e2 e1' e2' :
+    e1 ==>! e1' ->
+    e2 ==>! e2' ->
+    <{ s𝔹 (~if [b] then e1 else e2) }> ==>! <{ ~if [b] then s𝔹 e1' else s𝔹 e2' }>
+| ROIteIte b e1 e2 e3 e4 e1' e2' e3' e4' :
+    e1 ==>! e1' ->
+    e2 ==>! e2' ->
+    e3 ==>! e3' ->
+    e4 ==>! e4' ->
+    <{ if (~if [b] then e1 else e2) then e3 else e4 }> ==>!
+      <{ ~if [b] then (if e1' then e3' else e4') else (if e2' then e3' else e4') }>
+| ROIteProj b b' e1 e2 e1' e2' :
+    e1 ==>! e1' ->
+    e2 ==>! e2' ->
+    <{ π@b' (~if [b] then e1 else e2) }> ==>!
+      <{ ~if [b] then π@b' e1' else π@b' e2' }>
+| ROIteCase b e1 e2 e3 e4 e1' e2' e3' e4' L1 L2 :
+    e1 ==>! e1' ->
+    e2 ==>! e2' ->
+    (forall x, x ∉ L1 -> <{ e3^x }> ==>! <{ e3'^x }>) ->
+    (forall x, x ∉ L2 -> <{ e4^x }> ==>! <{ e4'^x }>) ->
+    <{ case (~if [b] then e1 else e2) of e3 | e4 }> ==>!
+      <{ ~if [b] then (case e1' of e3' | e4') else (case e2' of e3' | e4') }>
+| ROIteUnfold X b e1 e2 e1' e2' :
+    e1 ==>! e1' ->
+    e2 ==>! e2' ->
+    <{ unfold<X> (~if [b] then e1 else e2) }> ==>!
+      <{ ~if [b] then unfold<X> e1' else unfold<X> e2' }>
+| RTapeOIte b e1 e2 e1' e2' :
+    e1 ==>! e1' ->
+    e2 ==>! e2' ->
+    <{ tape (~if [b] then e1 else e2) }> ==>! <{ mux [b] (tape e1') (tape e2') }>
+| RTapePair e1 e2 e1' e2' :
+    e1 ==>! e1' ->
+    e2 ==>! e2' ->
+    woval e1 -> woval e2 ->
+    <{ tape (e1, e2) }> ==>! <{ (tape e1', tape e2') }>
+| RTapeUnitV :
+    <{ tape () }> ==>! <{ () }>
+| RTapeBoxedLit b :
+    <{ tape [b] }> ==>! <{ [b] }>
+| RTapeBoxedInj b ω v :
+    otval ω -> oval v ->
+    <{ tape [inj@b<ω> v] }> ==>! <{ [inj@b<ω> v] }>
 (* Congruence rules *)
 | RCgrProd τ1 τ2 τ1' τ2' :
     τ1 ==>! τ1' ->
@@ -148,14 +205,14 @@ not needed because they are not involved in type-level computation. *)
     τ1 ==>! τ1' ->
     τ2 ==>! τ2' ->
     <{ τ1 +{l} τ2 }> ==>! <{ τ1' +{l} τ2' }>
-| RCgrPi τ1 τ2 τ1' τ2' L :
+| RCgrPi l τ1 τ2 τ1' τ2' L :
     τ1 ==>! τ1' ->
     (forall x, x ∉ L -> <{ τ2^x }> ==>! <{ τ2'^x }>) ->
-    <{ Π:τ1, τ2 }> ==>! <{ Π:τ1', τ2' }>
-| RCgrAbs τ e τ' e' L :
+    <{ Π:{l}τ1, τ2 }> ==>! <{ Π:{l}τ1', τ2' }>
+| RCgrAbs l τ e τ' e' L :
     τ ==>! τ' ->
     (forall x, x ∉ L -> <{ e^x }> ==>! <{ e'^x }>) ->
-    <{ \:τ => e }> ==>! <{ \:τ' => e' }>
+    <{ \:{l}τ => e }> ==>! <{ \:{l}τ' => e' }>
 | RCgrApp e1 e2 e1' e2' :
     e1 ==>! e1' ->
     e2 ==>! e2' ->
@@ -194,6 +251,14 @@ not needed because they are not involved in type-level computation. *)
     (forall x, x ∉ L1 -> <{ e1^x }> ==>! <{ e1'^x }>) ->
     (forall x, x ∉ L2 -> <{ e2^x }> ==>! <{ e2'^x }>) ->
     <{ case{l} e0 of e1 | e2 }> ==>! <{ case{l} e0' of e1' | e2' }>
+| RCgrMux e0 e1 e2 e0' e1' e2' :
+    e0 ==>! e0' ->
+    e1 ==>! e1' ->
+    e2 ==>! e2' ->
+    <{ mux e0 e1 e2 }> ==>! <{ mux e0' e1' e2' }>
+| RCgrTape e e' :
+    e ==>! e' ->
+    <{ tape e }> ==>! <{ tape e' }>
 (* Reflexive rule *)
 | RRefl e :
     lc e ->
@@ -231,98 +296,114 @@ Inductive pared_equiv_join : expr -> expr -> Prop :=
 
 (** ** Expression typing and kinding *)
 (** They are mutually defined. *)
-Reserved Notation "Γ '⊢' e ':' τ" (at level 40,
-                                   e custom oadt at level 99,
-                                   τ custom oadt at level 99).
+Reserved Notation "Γ '⊢' e ':{' l '}' τ" (at level 40,
+                                          e custom oadt at level 99,
+                                          l constr at level 99,
+                                          τ custom oadt at level 99).
 Reserved Notation "Γ '⊢' τ '::' κ" (at level 40,
                                     τ custom oadt at level 99,
                                     κ custom oadt at level 99).
 
-Inductive typing : tctx -> expr -> expr -> Prop :=
-| TFVar Γ x τ κ :
-    Γ !! x = Some τ ->
+Inductive typing : tctx -> expr -> bool -> expr -> Prop :=
+| TFVar Γ x l τ κ :
+    Γ !! x = Some (l, τ) ->
     Γ ⊢ τ :: κ ->
-    Γ ⊢ fvar x : τ
-| TGVar Γ x τ e :
-    Σ !! x = Some (DFun τ e) ->
-    Γ ⊢ gvar x : τ
-| TAbs Γ e τ1 τ2 κ L :
-    (forall x, x ∉ L -> <[x:=τ2]>Γ ⊢ e^x : τ1^x) ->
+    Γ ⊢ fvar x :{l} τ
+| TGVar Γ x l τ e :
+    Σ !! x = Some (DFun (l, τ) e) ->
+    Γ ⊢ gvar x :{l} τ
+| TAbs Γ l1 l2 e τ1 τ2 κ L :
+    (forall x, x ∉ L -> <[x:=(l2, τ2)]>Γ ⊢ e^x :{l1} τ1^x) ->
     Γ ⊢ τ2 :: κ ->
-    Γ ⊢ \:τ2 => e : (Π:τ2, τ1)
-| TLet Γ e1 e2 τ1 τ2 L :
-    (forall x, x ∉ L -> <[x:=τ1]>Γ ⊢ e2^x : τ2^x) ->
-    Γ ⊢ e1 : τ1 ->
-    Γ ⊢ let e1 in e2 : τ2^e1
-| TApp Γ e1 e2 τ1 τ2 :
-    Γ ⊢ e1 : (Π:τ2, τ1) ->
-    Γ ⊢ e2 : τ2 ->
-    Γ ⊢ e1 e2 : τ1^e2
-| TUnit Γ : Γ ⊢ () : 𝟙
-| TLit Γ b : Γ ⊢ lit b : 𝔹
-| TSec Γ e :
-    Γ ⊢ e : 𝔹 ->
-    Γ ⊢ s𝔹 e : ~𝔹
-| TIte Γ e0 e1 e2 τ κ :
-    Γ ⊢ e0 : 𝔹 ->
-    Γ ⊢ e1 : τ^(lit true) ->
-    Γ ⊢ e2 : τ^(lit false) ->
+    Γ ⊢ \:{l2}τ2 => e :{l1} (Π:{l2}τ2, τ1)
+| TLet Γ l1 l2 l e1 e2 τ1 τ2 L :
+    (forall x, x ∉ L -> <[x:=(l1, τ1)]>Γ ⊢ e2^x :{l2} τ2^x) ->
+    Γ ⊢ e1 :{l1} τ1 ->
+    l = l1 ⊔ l2 ->
+    Γ ⊢ let e1 in e2 :{l} τ2^e1
+| TApp Γ l1 l2 e1 e2 τ1 τ2 :
+    Γ ⊢ e1 :{l1} (Π:{l2}τ2, τ1) ->
+    Γ ⊢ e2 :{l2} τ2 ->
+    Γ ⊢ e1 e2 :{l1} τ1^e2
+| TUnit Γ : Γ ⊢ () :{⊥} 𝟙
+| TLit Γ b : Γ ⊢ lit b :{⊥} 𝔹
+| TSec Γ l e :
+    Γ ⊢ e :{l} 𝔹 ->
+    Γ ⊢ s𝔹 e :{l} ~𝔹
+| TIte Γ l0 l1 l2 l e0 e1 e2 τ κ :
+    Γ ⊢ e0 :{l0} 𝔹 ->
+    Γ ⊢ e1 :{l1} τ^(lit true) ->
+    Γ ⊢ e2 :{l2} τ^(lit false) ->
     Γ ⊢ τ^e0 :: κ ->
-    Γ ⊢ if e0 then e1 else e2 : τ^e0
-| TMux Γ e0 e1 e2 τ :
-    Γ ⊢ e0 : ~𝔹 ->
-    Γ ⊢ e1 : τ ->
-    Γ ⊢ e2 : τ ->
-    Γ ⊢ τ :: *@O ->
-    Γ ⊢ ~if e0 then e1 else e2 : τ
-| TInj Γ b e τ1 τ2 κ :
-    Γ ⊢ e : ite b τ1 τ2 ->
+    l = l0 ⊔ l1 ⊔ l2 ->
+    Γ ⊢ if e0 then e1 else e2 :{l} τ^e0
+| TOIte Γ l1 l2 e0 e1 e2 τ κ :
+    Γ ⊢ e0 :{⊥} ~𝔹 ->
+    Γ ⊢ e1 :{l1} τ ->
+    Γ ⊢ e2 :{l2} τ ->
+    Γ ⊢ τ :: κ ->
+    Γ ⊢ ~if e0 then e1 else e2 :{⊤} τ
+| TInj Γ l b e τ1 τ2 κ :
+    Γ ⊢ e :{l} ite b τ1 τ2 ->
     Γ ⊢ τ1 + τ2 :: κ ->
-    Γ ⊢ inj@b<τ1 + τ2> e : τ1 + τ2
+    Γ ⊢ inj@b<τ1 + τ2> e :{l} τ1 + τ2
 | TOInj Γ b e τ1 τ2 :
-    Γ ⊢ e : ite b τ1 τ2 ->
+    Γ ⊢ e :{⊥} ite b τ1 τ2 ->
     Γ ⊢ τ1 ~+ τ2 :: *@O ->
-    Γ ⊢ ~inj@b<τ1 ~+ τ2> e : τ1 ~+ τ2
-| TCase Γ e0 e1 e2 τ1 τ2 τ κ L1 L2 :
-    (forall x, x ∉ L1 -> <[x:=τ1]>Γ ⊢ e1^x : τ^(inl<τ1 + τ2> x)) ->
-    (forall x, x ∉ L2 -> <[x:=τ2]>Γ ⊢ e2^x : τ^(inr<τ1 + τ2> x)) ->
-    Γ ⊢ e0 : τ1 + τ2 ->
+    Γ ⊢ ~inj@b<τ1 ~+ τ2> e :{⊥} τ1 ~+ τ2
+| TCase Γ l0 l1 l2 l e0 e1 e2 τ1 τ2 τ κ L1 L2 :
+    (forall x, x ∉ L1 -> <[x:=(l0, τ1)]>Γ ⊢ e1^x :{l1} τ^(inl<τ1 + τ2> x)) ->
+    (forall x, x ∉ L2 -> <[x:=(l0, τ2)]>Γ ⊢ e2^x :{l2} τ^(inr<τ1 + τ2> x)) ->
+    Γ ⊢ e0 :{l0} τ1 + τ2 ->
     Γ ⊢ τ^e0 :: κ ->
-    Γ ⊢ case e0 of e1 | e2 : τ^e0
-| TOCase Γ e0 e1 e2 τ1 τ2 τ L1 L2 :
-    (forall x, x ∉ L1 -> <[x:=τ1]>Γ ⊢ e1^x : τ) ->
-    (forall x, x ∉ L2 -> <[x:=τ2]>Γ ⊢ e2^x : τ) ->
-    Γ ⊢ e0 : τ1 ~+ τ2 ->
+    l = l0 ⊔ l1 ⊔ l2 ->
+    Γ ⊢ case e0 of e1 | e2 :{l} τ^e0
+| TOCase Γ l1 l2 e0 e1 e2 τ1 τ2 τ κ L1 L2 :
+    (forall x, x ∉ L1 -> <[x:=(⊥, τ1)]>Γ ⊢ e1^x :{l1} τ) ->
+    (forall x, x ∉ L2 -> <[x:=(⊥, τ2)]>Γ ⊢ e2^x :{l2} τ) ->
+    Γ ⊢ e0 :{⊥} τ1 ~+ τ2 ->
+    Γ ⊢ τ :: κ ->
+    Γ ⊢ ~case e0 of e1 | e2 :{⊤} τ
+| TPair Γ l1 l2 l e1 e2 τ1 τ2 :
+    Γ ⊢ e1 :{l1} τ1 ->
+    Γ ⊢ e2 :{l2} τ2 ->
+    l = l1 ⊔ l2 ->
+    Γ ⊢ (e1, e2) :{l} τ1 * τ2
+| TProj Γ l b e τ1 τ2 :
+    Γ ⊢ e :{l} τ1 * τ2 ->
+    Γ ⊢ π@b e :{l} ite b τ1 τ2
+| TFold Γ l X e τ :
+    Σ !! X = Some (DADT τ) ->
+    Γ ⊢ e :{l} τ ->
+    Γ ⊢ fold<X> e :{l} gvar X
+| TUnfold Γ l X e τ :
+    Σ !! X = Some (DADT τ) ->
+    Γ ⊢ e :{l} gvar X ->
+    Γ ⊢ unfold<X> e :{l} τ
+| TMux Γ e0 e1 e2 τ :
+    Γ ⊢ e0 :{⊥} ~𝔹 ->
+    Γ ⊢ e1 :{⊥} τ ->
+    Γ ⊢ e2 :{⊥} τ ->
     Γ ⊢ τ :: *@O ->
-    Γ ⊢ ~case e0 of e1 | e2 : τ
-| TPair Γ e1 e2 τ1 τ2 :
-    Γ ⊢ e1 : τ1 ->
-    Γ ⊢ e2 : τ2 ->
-    Γ ⊢ (e1, e2) : τ1 * τ2
-| TProj Γ b e τ1 τ2 :
-    Γ ⊢ e : τ1 * τ2 ->
-    Γ ⊢ π@b e : ite b τ1 τ2
-| TFold Γ X e τ :
-    Σ !! X = Some (DADT τ) ->
-    Γ ⊢ e : τ ->
-    Γ ⊢ fold<X> e : gvar X
-| TUnfold Γ X e τ :
-    Σ !! X = Some (DADT τ) ->
-    Γ ⊢ e : gvar X ->
-    Γ ⊢ unfold<X> e : τ
+    Γ ⊢ mux e0 e1 e2 :{⊥} τ
+| TTape Γ l e τ :
+    Γ ⊢ e :{l} τ ->
+    Γ ⊢ τ :: *@O ->
+    Γ ⊢ tape e :{⊥} τ
 (** Typing for runtime expressions is for metatheories. These expressions do not
 appear in source programs. Plus, it is not possible to type them at runtime
 since they are "encrypted" values. *)
-| TBoxedLit Γ b : Γ ⊢ [b] : ~𝔹
+| TBoxedLit Γ b : Γ ⊢ [b] :{⊥} ~𝔹
 | TBoxedInj Γ b v ω :
     ovalty <{ [inj@b<ω> v] }> ω ->
-    Γ ⊢ [inj@b<ω> v] : ω
+    Γ ⊢ [inj@b<ω> v] :{⊥} ω
 (** Type conversion *)
-| TConv Γ e τ τ' κ :
-    Γ ⊢ e : τ' ->
+| TConv Γ l l' e τ τ' κ :
+    Γ ⊢ e :{l'} τ' ->
     Γ ⊢ τ :: κ ->
     τ' ≡ τ ->
-    Γ ⊢ e : τ
+    l' ⊑ l ->
+    Γ ⊢ e :{l} τ
 
 with kinding : tctx -> expr -> kind -> Prop :=
 | KVarADT Γ X τ :
@@ -330,13 +411,13 @@ with kinding : tctx -> expr -> kind -> Prop :=
     Γ ⊢ gvar X :: *@P
 | KUnit Γ : Γ ⊢ 𝟙 :: *@A
 | KBool Γ l : Γ ⊢ 𝔹{l} :: ite l *@O *@P
-| KPi Γ τ1 τ2 κ1 κ2 L :
-    (forall x, x ∉ L -> <[x:=τ1]>Γ ⊢ τ2^x :: κ2) ->
+| KPi Γ l τ1 τ2 κ1 κ2 L :
+    (forall x, x ∉ L -> <[x:=(l, τ1)]>Γ ⊢ τ2^x :: κ2) ->
     Γ ⊢ τ1 :: κ1 ->
-    Γ ⊢ (Π:τ1, τ2) :: *@M
+    Γ ⊢ (Π:{l}τ1, τ2) :: *@M
 | KApp Γ e' e τ X :
     Σ !! X = Some (DOADT τ e') ->
-    Γ ⊢ e : τ ->
+    Γ ⊢ e :{⊥} τ ->
     Γ ⊢ (gvar X) e :: *@O
 | KProd Γ τ1 τ2 κ :
     Γ ⊢ τ1 :: κ ->
@@ -351,25 +432,26 @@ with kinding : tctx -> expr -> kind -> Prop :=
     Γ ⊢ τ2 :: *@O ->
     Γ ⊢ τ1 ~+ τ2 :: *@O
 | KIte Γ e0 τ1 τ2 :
-    Γ ⊢ e0 : 𝔹 ->
+    Γ ⊢ e0 :{⊥} 𝔹 ->
     Γ ⊢ τ1 :: *@O ->
     Γ ⊢ τ2 :: *@O ->
     Γ ⊢ if e0 then τ1 else τ2 :: *@O
 | KCase Γ e0 τ1 τ2 τ1' τ2' L1 L2 :
-    (forall x, x ∉ L1 -> <[x:=τ1']>Γ ⊢ τ1^x :: *@O) ->
-    (forall x, x ∉ L2 -> <[x:=τ2']>Γ ⊢ τ2^x :: *@O) ->
-    Γ ⊢ e0 : τ1' + τ2' ->
+    (forall x, x ∉ L1 -> <[x:=(⊥, τ1')]>Γ ⊢ τ1^x :: *@O) ->
+    (forall x, x ∉ L2 -> <[x:=(⊥, τ2')]>Γ ⊢ τ2^x :: *@O) ->
+    Γ ⊢ e0 :{⊥} τ1' + τ2' ->
     Γ ⊢ case e0 of τ1 | τ2 :: *@O
 | KLet Γ e τ τ' L :
-    (forall x, x ∉ L -> <[x:=τ']>Γ ⊢ τ^x :: *@O) ->
-    Γ ⊢ e : τ' ->
+    (forall x, x ∉ L -> <[x:=(⊥, τ')]>Γ ⊢ τ^x :: *@O) ->
+    Γ ⊢ e :{⊥} τ' ->
     Γ ⊢ let e in τ :: *@O
 | KSub Γ τ κ κ' :
     Γ ⊢ τ :: κ' ->
     κ' ⊑ κ ->
     Γ ⊢ τ :: κ
 
-where "Γ '⊢' e ':' τ" := (typing Γ e τ) and "Γ '⊢' τ '::' κ" := (kinding Γ τ κ)
+where "Γ '⊢' e ':{' l '}' τ" := (typing Γ e l τ)
+  and "Γ '⊢' τ '::' κ" := (kinding Γ τ κ)
 .
 
 End fix_gctx.
@@ -378,11 +460,12 @@ Notation "Σ '⊢' e '≡' e'" := (pared_equiv Σ e e')
                                (at level 40,
                                 e custom oadt at level 99,
                                 e' custom oadt at level 99).
-Notation "Σ ; Γ '⊢' e ':' τ" := (typing Σ Γ e τ)
-                                  (at level 40,
-                                   Γ constr at level 0,
-                                   e custom oadt at level 99,
-                                   τ custom oadt at level 99).
+Notation "Σ ; Γ '⊢' e ':{' l '}' τ" := (typing Σ Γ e l τ)
+                                         (at level 40,
+                                          Γ constr at level 0,
+                                          e custom oadt at level 99,
+                                          τ custom oadt at level 99,
+                                          format "Σ ;  Γ  '⊢'  e  ':{' l '}'  τ").
 Notation "Σ ; Γ '⊢' τ '::' κ" := (kinding Σ Γ τ κ)
                                    (at level 40,
                                     Γ constr at level 0,
@@ -399,12 +482,12 @@ Inductive gdef_typing : gctx -> gdef -> Prop :=
     Σ ⊢₁ (DADT τ)
 | TOADT Σ X τ e L :
     Σ; ∅ ⊢ τ :: *@P ->
-    (forall x, x ∉ L -> Σ; ({[x:=τ]}) ⊢ e^x :: *@O) ->
+    (forall x, x ∉ L -> Σ; ({[x:=(⊥, τ)]}) ⊢ e^x :: *@O) ->
     Σ ⊢₁ (DOADT τ e)
-| TFun Σ X τ e κ :
+| TFun Σ X l τ e κ :
     Σ; ∅ ⊢ τ :: κ ->
-    Σ; ∅ ⊢ e : τ ->
-    Σ ⊢₁ (DFun τ e)
+    Σ; ∅ ⊢ e :{l} τ ->
+    Σ ⊢₁ (DFun (l, τ) e)
 
 where "Σ '⊢₁' D" := (gdef_typing Σ D)
 .
@@ -414,7 +497,7 @@ Definition gctx_typing (Σ : gctx) : Prop :=
 
 (** ** Program typing *)
 Definition program_typing (Σ : gctx) (e : expr) (τ : expr) :=
-  gctx_typing Σ /\ Σ; ∅ ⊢ e : τ.
+  gctx_typing Σ /\ Σ; ∅ ⊢ e :{⊥} τ.
 
 (** ** Well-formedness of [gctx] *)
 (* Equivalent to [gctx_typing]. Essentially saying all definitions in [Σ] are
@@ -426,9 +509,9 @@ Definition gctx_wf (Σ : gctx) :=
                   Σ; ∅ ⊢ τ :: *@P
                 | DOADT τ e =>
                   Σ; ∅ ⊢ τ :: *@P /\
-                  exists L, forall x, x ∉ L -> Σ; ({[x:=τ]}) ⊢ e^x :: *@O
-                | DFun τ e =>
-                  Σ; ∅ ⊢ e : τ /\
+                  exists L, forall x, x ∉ L -> Σ; ({[x:=(⊥, τ)]}) ⊢ e^x :: *@O
+                | DFun (l, τ) e =>
+                  Σ; ∅ ⊢ e :{l} τ /\
                   exists κ, Σ; ∅ ⊢ τ :: κ
                 end) Σ.
 
@@ -459,11 +542,19 @@ Notation "Σ '⊢' e '≡' e'" := (pared_equiv Σ e e')
                                 e custom oadt at level 99,
                                 e' custom oadt at level 99).
 
-Notation "Σ ; Γ '⊢' e ':' τ" := (typing Σ Γ e τ)
-                                  (at level 40,
-                                   Γ constr at level 0,
-                                   e custom oadt at level 99,
-                                   τ custom oadt at level 99).
+Notation "Σ ; Γ '⊢' e ':{' l '}' τ" := (typing Σ Γ e l τ)
+                                         (at level 40,
+                                          Γ constr at level 0,
+                                          e custom oadt at level 99,
+                                          l constr at level 99,
+                                          τ custom oadt at level 99,
+                                          format "Σ ;  Γ  '⊢'  e  ':{' l '}'  τ").
+Notation "Σ ; Γ '⊢' e ':' τ" := (typing Σ Γ e _ τ)
+                                         (at level 40,
+                                          Γ constr at level 0,
+                                          e custom oadt at level 99,
+                                          τ custom oadt at level 99,
+                                          only parsing).
 Notation "Σ ; Γ '⊢' τ '::' κ" := (kinding Σ Γ τ κ)
                                    (at level 40,
                                     Γ constr at level 0,
