theories/lang_oadt/inversion.v
@@ -22,6 +22,9 @@ Section inversion.
 Context (Σ : gctx).
 Context (Hwf : gctx_wf Σ).
 
+#[local]
+Set Default Proof Using "Type".
+
 (** ** Kind inversion  *)
 Tactic Notation "kind_inv_solver" "by" tactic3(tac) :=
   match goal with
@@ -30,17 +33,18 @@ Tactic Notation "kind_inv_solver" "by" tactic3(tac) :=
   induction 1; subst; simp_hyps; simplify_eq;
   tac.
 
-Tactic Notation "kind_inv_solver" :=
-  kind_inv_solver by (repeat esplit; eauto; lattice_naive_solver).
+Ltac kind_inv_solver :=
+  kind_inv_solver by (repeat esplit; eauto;
+                      lattice_naive_solver by eauto using top_inv, join_ub_r).
 
-Lemma kind_inv_pi Γ τ1 τ2 κ :
-  Σ; Γ ⊢ Π:τ1, τ2 :: κ ->
+Lemma kind_inv_pi Γ l τ1 τ2 κ :
+  Σ; Γ ⊢ Π:{l}τ1, τ2 :: κ ->
   κ = <{ *@M }> /\
   exists L κ1 κ2,
-    (∀ x, x ∉ L → Σ; (<[x:=τ1]> Γ) ⊢ τ2^x :: κ2) /\
+    (∀ x, x ∉ L → Σ; (<[x:=(l, τ1)]> Γ) ⊢ τ2^x :: κ2) /\
     Σ; Γ ⊢ τ1 :: κ1.
 Proof.
-  kind_inv_solver by sfirstorder use: top_inv.
+  kind_inv_solver.
 Qed.
 
 Lemma kind_inv_bool Γ κ :
@@ -66,8 +70,7 @@ Lemma kind_inv_sum Γ τ1 τ2 κ :
     Σ; Γ ⊢ τ1 :: κ' /\
     Σ; Γ ⊢ τ2 :: κ'.
 Proof.
-  kind_inv_solver by qauto l: on solve: lattice_naive_solver
-                           use: join_ub_r.
+  kind_inv_solver.
 Qed.
 
 Lemma kind_inv_osum Γ τ1 τ2 κ :
@@ -91,7 +94,7 @@ Lemma kind_inv_app Γ e1 e2 κ :
   <{ *@O }> ⊑ κ /\
   exists X τ e',
     Σ !! X = Some (DOADT τ e') /\
-    Σ; Γ ⊢ e2 : τ /\
+    Σ; Γ ⊢ e2 :{⊥} τ /\
     e1 = <{ gvar X }>.
 Proof.
   kind_inv_solver.
@@ -101,7 +104,7 @@ Lemma kind_inv_ite Γ l e0 τ1 τ2 κ :
   Σ; Γ ⊢ if{l} e0 then τ1 else τ2 :: κ ->
   <{ *@O }> ⊑ κ /\
   l = low /\
-  Σ; Γ ⊢ e0 : 𝔹 /\
+  Σ; Γ ⊢ e0 :{⊥} 𝔹 /\
   Σ; Γ ⊢ τ1 :: *@O /\
   Σ; Γ ⊢ τ2 :: *@O.
 Proof.
@@ -112,8 +115,8 @@ Lemma kind_inv_let Γ e τ κ :
   Σ; Γ ⊢ let e in τ :: κ ->
   <{ *@O }> ⊑ κ /\
   exists τ' L,
-    Σ; Γ ⊢ e : τ' /\
-    (forall x, x ∉ L -> Σ; (<[x:=τ']> Γ) ⊢ τ^x :: *@O).
+    Σ; Γ ⊢ e :{⊥} τ' /\
+    (forall x, x ∉ L -> Σ; (<[x:=(⊥, τ')]> Γ) ⊢ τ^x :: *@O).
 Proof.
   kind_inv_solver.
 Qed.
@@ -123,15 +126,21 @@ Lemma kind_inv_case Γ l e0 τ1 τ2 κ :
   <{ *@O }> ⊑ κ /\
   l = low /\
   exists τ1' τ2' L1 L2,
-    Σ; Γ ⊢ e0 : τ1' + τ2' /\
-    (forall x, x ∉ L1 -> Σ; (<[x:=τ1']> Γ) ⊢ τ1^x :: *@O) /\
-    (forall x, x ∉ L2 -> Σ; (<[x:=τ2']> Γ) ⊢ τ2^x :: *@O).
+    Σ; Γ ⊢ e0 :{⊥} τ1' + τ2' /\
+    (forall x, x ∉ L1 -> Σ; (<[x:=(⊥, τ1')]> Γ) ⊢ τ1^x :: *@O) /\
+    (forall x, x ∉ L2 -> Σ; (<[x:=(⊥, τ2')]> Γ) ⊢ τ2^x :: *@O).
+Proof.
+  kind_inv_solver.
+Qed.
+
+Lemma kind_inv_oite Γ e0 e1 e2 κ :
+  Σ; Γ ⊢ ~if e0 then e1 else e2 :: κ -> False.
 Proof.
   kind_inv_solver.
 Qed.
 
 Lemma kind_inv_mux Γ e0 e1 e2 κ :
-  Σ; Γ ⊢ ~if e0 then e1 else e2 :: κ -> False.
+  Σ; Γ ⊢ mux e0 e1 e2 :: κ -> False.
 Proof.
   kind_inv_solver.
 Qed.
@@ -178,8 +187,14 @@ Proof.
   kind_inv_solver.
 Qed.
 
-Lemma kind_inv_abs Γ τ e κ :
-  Σ; Γ ⊢ \:τ => e :: κ -> False.
+Lemma kind_inv_abs Γ l τ e κ :
+  Σ; Γ ⊢ \:{l}τ => e :: κ -> False.
+Proof.
+  kind_inv_solver.
+Qed.
+
+Lemma kind_inv_tape Γ e κ :
+  Σ; Γ ⊢ tape e :: κ -> False.
 Proof.
   kind_inv_solver.
 Qed.
@@ -192,93 +207,118 @@ Tactic Notation "type_inv_solver" "by" tactic3(tac) :=
   induction 1; subst; simp_hyps; simplify_eq;
   tac.
 
-Tactic Notation "type_inv_solver" :=
-  type_inv_solver by (repeat esplit; eauto; equiv_naive_solver).
+Ltac type_inv_solver :=
+  type_inv_solver by (repeat (eauto; esplit);
+                      try first [ goal_is (_ ⊢ _ ≡ _); equiv_naive_solver
+                                | try select kind (fun k => clear dependent k);
+                                  lattice_naive_solver
+                                    by eauto using (top_inv (A:=bool)) ]).
 
-Lemma type_inv_unit Γ τ :
-  Σ; Γ ⊢ () : τ ->
+Lemma type_inv_prod Γ l τ1 τ2 τ :
+  Σ; Γ ⊢ τ1 * τ2 :{l} τ -> False.
+Proof.
+  type_inv_solver.
+Qed.
+
+Lemma type_inv_sum Γ l l' τ1 τ2 τ :
+  Σ; Γ ⊢ τ1 +{l} τ2 :{l'} τ -> False.
+Proof.
+  type_inv_solver.
+Qed.
+
+#[local]
+Set Default Proof Using "Hwf".
+
+Lemma type_inv_unit Γ l τ :
+  Σ; Γ ⊢ () :{l} τ ->
+  ⊥ ⊑ l /\
   Σ ⊢ τ ≡ 𝟙.
 Proof.
   type_inv_solver.
 Qed.
 
-Lemma type_inv_lit Γ b τ :
-  Σ; Γ ⊢ lit b : τ ->
+Lemma type_inv_lit Γ l b τ :
+  Σ; Γ ⊢ lit b :{l} τ ->
   Σ ⊢ τ ≡ 𝔹.
 Proof.
   type_inv_solver.
 Qed.
 
-Lemma type_inv_abs Γ e τ2 τ :
-  Σ; Γ ⊢ \:τ2 => e : τ ->
-  exists τ1 κ L,
+Lemma type_inv_abs Γ l1 l2 e τ2 τ :
+  Σ; Γ ⊢ \:{l2}τ2 => e :{l1} τ ->
+  exists l1' τ1 κ L,
     Σ; Γ ⊢ τ2 :: κ /\
-    (forall x, x ∉ L -> Σ; (<[x:=τ2]> Γ) ⊢ e^x : τ1^x) /\
-    Σ ⊢ τ ≡ Π:τ2, τ1.
+    (forall x, x ∉ L -> Σ; (<[x:=(l2, τ2)]> Γ) ⊢ e^x :{l1'} τ1^x) /\
+    l1' ⊑ l1 /\
+    Σ ⊢ τ ≡ Π:{l2}τ2, τ1.
 Proof.
   type_inv_solver.
 Qed.
 
-Lemma type_inv_gvar Γ x τ :
-  Σ; Γ ⊢ gvar x : τ ->
-  exists τ' e,
-    Σ !! x = Some (DFun τ' e) /\
+Lemma type_inv_gvar Γ l x τ :
+  Σ; Γ ⊢ gvar x :{l} τ ->
+  exists l' τ' e,
+    Σ !! x = Some (DFun (l', τ') e) /\
+    l' ⊑ l /\
     Σ ⊢ τ ≡ τ'.
 Proof.
   type_inv_solver.
 Qed.
 
-Lemma type_inv_pair Γ e1 e2 τ :
-  Σ; Γ ⊢ (e1, e2) : τ ->
-  exists τ1 τ2,
-    Σ; Γ ⊢ e1 : τ1 /\
-    Σ; Γ ⊢ e2 : τ2 /\
+Lemma type_inv_pair Γ l e1 e2 τ :
+  Σ; Γ ⊢ (e1, e2) :{l} τ ->
+  exists l1 l2 τ1 τ2,
+    Σ; Γ ⊢ e1 :{l1} τ1 /\
+    Σ; Γ ⊢ e2 :{l2} τ2 /\
+    l1 ⊔ l2 ⊑ l /\
     Σ ⊢ τ ≡ τ1 * τ2.
 Proof.
   type_inv_solver.
 Qed.
 
-Lemma type_inv_inj Γ b e τ' τ :
-  Σ; Γ ⊢ inj@b<τ'> e : τ ->
-  exists τ1 τ2 κ,
+Lemma type_inv_inj Γ l b e τ' τ :
+  Σ; Γ ⊢ inj@b<τ'> e :{l} τ ->
+  exists l' τ1 τ2 κ,
     τ' = <{ τ1 + τ2 }> /\
     Σ; Γ ⊢ τ1 + τ2 :: κ /\
-    Σ; Γ ⊢ e : ite b τ1 τ2 /\
+    Σ; Γ ⊢ e :{l'} ite b τ1 τ2 /\
+    l' ⊑ l /\
     Σ ⊢ τ ≡ τ1 + τ2.
 Proof.
   type_inv_solver.
 Qed.
 
-Lemma type_inv_oinj Γ b e τ' τ :
-  Σ; Γ ⊢ ~inj@b<τ'> e : τ ->
+Lemma type_inv_oinj Γ l b e τ' τ :
+  Σ; Γ ⊢ ~inj@b<τ'> e :{l} τ ->
   exists τ1 τ2,
     τ' = <{ τ1 ~+ τ2 }> /\
     Σ; Γ ⊢ τ1 ~+ τ2 :: *@O /\
-    Σ; Γ ⊢ e : ite b τ1 τ2 /\
+    Σ; Γ ⊢ e :{⊥} ite b τ1 τ2 /\
     Σ ⊢ τ ≡ τ1 ~+ τ2.
 Proof.
   type_inv_solver.
 Qed.
 
-Lemma type_inv_fold Γ X e τ :
-  Σ; Γ ⊢ fold<X> e : τ ->
-  exists τ',
-    Σ; Γ ⊢ e : τ' /\
+Lemma type_inv_fold Γ l X e τ :
+  Σ; Γ ⊢ fold<X> e :{l} τ ->
+  exists l' τ',
+    Σ; Γ ⊢ e :{l'} τ' /\
     Σ !! X = Some (DADT τ') /\
+    l' ⊑ l /\
     Σ ⊢ τ ≡ gvar X.
 Proof.
   type_inv_solver.
 Qed.
 
-Lemma type_inv_boxedlit Γ b τ :
-  Σ; Γ ⊢ [b] : τ ->
+Lemma type_inv_boxedlit Γ l b τ :
+  Σ; Γ ⊢ [b] :{l} τ ->
   Σ ⊢ τ ≡ ~𝔹.
 Proof.
   type_inv_solver.
 Qed.
 
-Lemma type_inv_boxedinj Γ b v ω τ :
-  Σ; Γ ⊢ [inj@b<ω> v] : τ ->
+Lemma type_inv_boxedinj Γ l b v ω τ :
+  Σ; Γ ⊢ [inj@b<ω> v] :{l} τ ->
   exists ω1 ω2,
     ω = <{ ω1 ~+ ω2 }> /\
     ovalty <{ [inj@b<ω> v] }> ω /\
@@ -288,120 +328,139 @@ Proof.
                            ctrs: ovalty inv: ovalty.
 Qed.
 
-Lemma type_inv_case Γ e0 e1 e2 τ :
-  Σ; Γ ⊢ case e0 of e1 | e2 : τ ->
-  exists τ1 τ2 τ' κ L1 L2,
+Lemma type_inv_case Γ l e0 e1 e2 τ :
+  Σ; Γ ⊢ case e0 of e1 | e2 :{l} τ ->
+  exists l0 l1 l2 τ1 τ2 τ' κ L1 L2,
     Σ; Γ ⊢ τ'^e0 :: κ /\
-    Σ; Γ ⊢ e0 : τ1 + τ2 /\
-    (forall x, x ∉ L1 -> Σ; (<[x:=τ1]> Γ) ⊢ e1^x : τ'^(inl<τ1 + τ2> x)) /\
-    (forall x, x ∉ L2 -> Σ; (<[x:=τ2]> Γ) ⊢ e2^x : τ'^(inr<τ1 + τ2> x)) /\
+    Σ; Γ ⊢ e0 :{l0} τ1 + τ2 /\
+    (forall x, x ∉ L1 -> Σ; (<[x:=(l0, τ1)]> Γ) ⊢ e1^x :{l1} τ'^(inl<τ1 + τ2> x)) /\
+    (forall x, x ∉ L2 -> Σ; (<[x:=(l0, τ2)]> Γ) ⊢ e2^x :{l2} τ'^(inr<τ1 + τ2> x)) /\
+    l0 ⊔ l1 ⊔ l2 ⊑ l /\
     Σ ⊢ τ ≡ τ'^e0.
 Proof.
   type_inv_solver.
 Qed.
 
-Lemma type_inv_ocase Γ e0 e1 e2 τ :
-  Σ; Γ ⊢ ~case e0 of e1 | e2 : τ ->
-  exists τ1 τ2 τ' L1 L2,
-    Σ; Γ ⊢ τ' :: *@O /\
-    Σ; Γ ⊢ e0 : τ1 ~+ τ2 /\
-    (forall x, x ∉ L1 -> Σ; (<[x:=τ1]> Γ) ⊢ e1^x : τ') /\
-    (forall x, x ∉ L2 -> Σ; (<[x:=τ2]> Γ) ⊢ e2^x : τ') /\
-    Σ ⊢ τ ≡ τ'.
-Proof.
-  type_inv_solver.
-Qed.
-
-Lemma type_inv_case_ Γ l e0 e1 e2 τ :
-  Σ; Γ ⊢ case{l} e0 of e1 | e2 : τ ->
-  exists τ1 τ2 τ' κ L1 L2,
+Lemma type_inv_ocase Γ l e0 e1 e2 τ :
+  Σ; Γ ⊢ ~case e0 of e1 | e2 :{l} τ ->
+  exists l1 l2 τ1 τ2 τ' κ L1 L2,
     Σ; Γ ⊢ τ' :: κ /\
-    Σ; Γ ⊢ e0 : τ1 +{l} τ2 /\
-    (forall x, x ∉ L1 -> exists τ', Σ; (<[x:=τ1]> Γ) ⊢ e1^x : τ') /\
-    (forall x, x ∉ L2 -> exists τ', Σ; (<[x:=τ2]> Γ) ⊢ e2^x : τ') /\
+    Σ; Γ ⊢ e0 :{⊥} τ1 ~+ τ2 /\
+    (forall x, x ∉ L1 -> Σ; (<[x:=(⊥, τ1)]> Γ) ⊢ e1^x :{l1} τ') /\
+    (forall x, x ∉ L2 -> Σ; (<[x:=(⊥, τ2)]> Γ) ⊢ e2^x :{l2} τ') /\
     Σ ⊢ τ ≡ τ'.
 Proof.
-  type_inv_solver by (repeat (esplit; eauto); equiv_naive_solver).
+  type_inv_solver.
 Qed.
 
-Lemma type_inv_prod Γ τ1 τ2 τ :
-  Σ; Γ ⊢ τ1 * τ2 : τ -> False.
+Lemma type_inv_case_ Γ l l' e0 e1 e2 τ :
+  Σ; Γ ⊢ case{l} e0 of e1 | e2 :{l'} τ ->
+  exists l0 l1 l2 τ1 τ2 τ' κ L1 L2,
+    Σ; Γ ⊢ τ' :: κ /\
+    Σ; Γ ⊢ e0 :{l0} τ1 +{l} τ2 /\
+    (forall x, x ∉ L1 -> exists τ', Σ; (<[x:=(l0, τ1)]> Γ) ⊢ e1^x :{l1} τ') /\
+    (forall x, x ∉ L2 -> exists τ', Σ; (<[x:=(l0, τ2)]> Γ) ⊢ e2^x :{l2} τ') /\
+    Σ ⊢ τ ≡ τ'.
 Proof.
   type_inv_solver.
 Qed.
 
-Lemma type_inv_sum Γ l τ1 τ2 τ :
-  Σ; Γ ⊢ τ1 +{l} τ2 : τ -> False.
-Proof.
-  type_inv_solver.
-Qed.
-
-Lemma type_inv_app Γ e1 e2 τ :
-  Σ; Γ ⊢ e1 e2 : τ ->
-  exists τ1 τ2,
-    Σ; Γ ⊢ e1 : Π:τ2, τ1 /\
-    Σ; Γ ⊢ e2 : τ2 /\
+Lemma type_inv_app Γ l1 e1 e2 τ :
+  Σ; Γ ⊢ e1 e2 :{l1} τ ->
+  exists l1' l2 τ1 τ2,
+    Σ; Γ ⊢ e1 :{l1'} Π:{l2}τ2, τ1 /\
+    Σ; Γ ⊢ e2 :{l2} τ2 /\
+    l1' ⊑ l1 /\
     Σ ⊢ τ ≡ τ1^e2.
 Proof.
   type_inv_solver.
 Qed.
 
-Lemma type_inv_let Γ e1 e2 τ :
-  Σ; Γ ⊢ let e1 in e2 : τ ->
-  exists τ1 τ2 L,
-    Σ; Γ ⊢ e1 : τ1 /\
-    (forall x, x ∉ L -> Σ; (<[x:=τ1]> Γ) ⊢ e2^x : τ2^x) /\
+Lemma type_inv_let Γ l e1 e2 τ :
+  Σ; Γ ⊢ let e1 in e2 :{l} τ ->
+  exists l1 l2 τ1 τ2 L,
+    Σ; Γ ⊢ e1 :{l1} τ1 /\
+    (forall x, x ∉ L -> Σ; (<[x:=(l1, τ1)]> Γ) ⊢ e2^x :{l2} τ2^x) /\
+    l1 ⊔ l2 ⊑ l /\
     Σ ⊢ τ ≡ τ2^e1.
 Proof.
   type_inv_solver.
 Qed.
 
-Lemma type_inv_sec Γ e τ :
-  Σ; Γ ⊢ s𝔹 e : τ ->
-  Σ; Γ ⊢ e : 𝔹 /\
-  Σ ⊢ τ ≡ ~𝔹.
+Lemma type_inv_sec Γ l e τ :
+  Σ; Γ ⊢ s𝔹 e :{l} τ ->
+  exists l',
+    Σ; Γ ⊢ e :{l'} 𝔹 /\
+    l' ⊑ l /\
+    Σ ⊢ τ ≡ ~𝔹.
 Proof.
   type_inv_solver.
 Qed.
 
-Lemma type_inv_ite Γ e0 e1 e2 τ :
-  Σ; Γ ⊢ if e0 then e1 else e2 : τ ->
-  exists τ' κ,
-    Σ; Γ ⊢ e0 : 𝔹 /\
-    Σ; Γ ⊢ e1 : τ'^(lit true) /\
-    Σ; Γ ⊢ e2 : τ'^(lit false) /\
+Lemma type_inv_ite Γ l e0 e1 e2 τ :
+  Σ; Γ ⊢ if e0 then e1 else e2 :{l} τ ->
+  exists l0 l1 l2 τ' κ,
+    Σ; Γ ⊢ e0 :{l0} 𝔹 /\
+    Σ; Γ ⊢ e1 :{l1} τ'^(lit true) /\
+    Σ; Γ ⊢ e2 :{l2} τ'^(lit false) /\
     Σ; Γ ⊢ τ'^e0 :: κ /\
+    l0 ⊔ l1 ⊔ l2 ⊑ l /\
     Σ ⊢ τ ≡ τ'^e0.
 Proof.
   type_inv_solver.
 Qed.
 
-Lemma type_inv_mux Γ e0 e1 e2 τ :
-  Σ; Γ ⊢ ~if e0 then e1 else e2 : τ ->
+Lemma type_inv_oite Γ l e0 e1 e2 τ :
+  Σ; Γ ⊢ ~if e0 then e1 else e2 :{l} τ ->
+  exists l1 l2 τ' κ,
+    Σ; Γ ⊢ e0 :{⊥} ~𝔹 /\
+    Σ; Γ ⊢ e1 :{l1} τ' /\
+    Σ; Γ ⊢ e2 :{l2} τ' /\
+    Σ; Γ ⊢ τ' :: κ /\
+    l = ⊤ /\
+    Σ ⊢ τ ≡ τ'.
+Proof.
+  type_inv_solver.
+Qed.
+
+Lemma type_inv_mux Γ l e0 e1 e2 τ :
+  Σ; Γ ⊢ mux e0 e1 e2 :{l} τ ->
   exists τ',
-    Σ; Γ ⊢ e0 : ~𝔹 /\
-    Σ; Γ ⊢ e1 : τ' /\
-    Σ; Γ ⊢ e2 : τ' /\
+    Σ; Γ ⊢ e0 :{⊥} ~𝔹 /\
+    Σ; Γ ⊢ e1 :{⊥} τ' /\
+    Σ; Γ ⊢ e2 :{⊥} τ' /\
     Σ; Γ ⊢ τ' :: *@O /\
     Σ ⊢ τ ≡ τ'.
 Proof.
   type_inv_solver.
 Qed.
 
-Lemma type_inv_proj Γ b e τ :
-  Σ; Γ ⊢ π@b e : τ ->
-  exists τ1 τ2,
-    Σ; Γ ⊢ e : τ1 * τ2 /\
+Lemma type_inv_proj Γ l b e τ :
+  Σ; Γ ⊢ π@b e :{l} τ ->
+  exists l' τ1 τ2,
+    Σ; Γ ⊢ e :{l'} τ1 * τ2 /\
+    l' ⊑ l /\
     Σ ⊢ τ ≡ ite b τ1 τ2.
 Proof.
   type_inv_solver.
 Qed.
 
-Lemma type_inv_unfold Γ X e τ :
-  Σ; Γ ⊢ unfold<X> e : τ ->
-  exists τ',
+Lemma type_inv_unfold Γ l X e τ :
+  Σ; Γ ⊢ unfold<X> e :{l} τ ->
+  exists l' τ',
     Σ !! X = Some (DADT τ') /\
-    Σ; Γ ⊢ e : gvar X /\
+    Σ; Γ ⊢ e :{l'} gvar X /\
+    l' ⊑ l /\
+    Σ ⊢ τ ≡ τ'.
+Proof.
+  type_inv_solver.
+Qed.
+
+Lemma type_inv_tape Γ l e τ :
+  Σ; Γ ⊢ tape e :{l} τ ->
+  exists l' τ',
+    Σ; Γ ⊢ e :{l'} τ' /\
+    Σ; Γ ⊢ τ' :: *@O /\
     Σ ⊢ τ ≡ τ'.
 Proof.
   type_inv_solver.
@@ -411,7 +470,7 @@ End inversion.
 
 Tactic Notation "apply_kind_inv" hyp(H) "by" tactic3(tac) :=
   lazymatch type of H with
-  | _; _ ⊢ Π:_, _ :: _ => tac kind_inv_pi
+  | _; _ ⊢ Π:{_}_, _ :: _ => tac kind_inv_pi
   | _; _ ⊢ 𝔹 :: _ => tac kind_inv_bool
   | _; _ ⊢ _ _ :: _ => tac kind_inv_app
   | _; _ ⊢ let _ in _ :: _ => tac kind_inv_let
@@ -419,7 +478,7 @@ Tactic Notation "apply_kind_inv" hyp(H) "by" tactic3(tac) :=
   | _; _ ⊢ _ + _ :: _ => tac kind_inv_sum
   | _; _ ⊢ _ ~+ _ :: _ => tac kind_inv_osum
   | _; _ ⊢ gvar _ :: _ => tac kind_inv_gvar
-  | _; _ ⊢ ~if _ then _ else _ :: _ => apply kind_inv_mux in H; elim H
+  | _; _ ⊢ ~if _ then _ else _ :: _ => apply kind_inv_oite in H; elim H
   | _; _ ⊢ if{_} _ then _ else _ :: _ => tac kind_inv_ite
   | _; _ ⊢ ~case _ of _ | _ :: _ => apply kind_inv_ocase in H; elim H
   | _; _ ⊢ case{_} _ of _ | _ :: _ => tac kind_inv_case
@@ -429,7 +488,9 @@ Tactic Notation "apply_kind_inv" hyp(H) "by" tactic3(tac) :=
   | _; _ ⊢ inj{_}@_<_> _ :: _ => apply kind_inv_inj in H; elim H
   | _; _ ⊢ fold<_> _ :: _ => apply kind_inv_fold in H; elim H
   | _; _ ⊢ unfold<_> _ :: _ => apply kind_inv_unfold in H; elim H
-  | _; _ ⊢ \:_ => _ :: _ => apply kind_inv_abs in H; elim H
+  | _; _ ⊢ \:{_}_ => _ :: _ => apply kind_inv_abs in H; elim H
+  | _; _ ⊢ mux _ _ _ :: _ => apply kind_inv_mux in H; elim H
+  | _; _ ⊢ tape _ :: _ => apply kind_inv_tape in H; elim H
   end.
 
 Tactic Notation "apply_kind_inv" hyp(H) :=
@@ -446,7 +507,7 @@ Tactic Notation "apply_type_inv" hyp(H) "by" tactic3(tac) :=
   | _; _ ⊢ () : _ => tac type_inv_unit
   | _; _ ⊢ lit _ : _ => tac type_inv_lit
   | _; _ ⊢ gvar _ : _ => tac type_inv_gvar
-  | _; _ ⊢ \:_ => _ : _ => tac type_inv_abs
+  | _; _ ⊢ \:{_}_ => _ : _ => tac type_inv_abs
   | _; _ ⊢ _ _ : _ => tac type_inv_app
   | _; _ ⊢ let _ in _ : _ => tac type_inv_let
   | _; _ ⊢ (_, _) : _ => tac type_inv_pair
@@ -454,13 +515,15 @@ Tactic Notation "apply_type_inv" hyp(H) "by" tactic3(tac) :=
   | _; _ ⊢ π@_ _ : _ => tac type_inv_proj
   | _; _ ⊢ ~inj@_<_> _ : _ => tac type_inv_oinj
   | _; _ ⊢ inj@_<_> _ : _ => tac type_inv_inj
-  | _; _ ⊢ ~if _ then _ else _ : _ => tac type_inv_mux
+  | _; _ ⊢ ~if _ then _ else _ : _ => tac type_inv_oite
   | _; _ ⊢ if _ then _ else _ : _ => tac type_inv_ite
   | _; _ ⊢ ~case _ of _ | _ : _ => tac type_inv_ocase
   | _; _ ⊢ case _ of _ | _ : _ => tac type_inv_case
   | _; _ ⊢ case{_} _ of _ | _ : _ => tac type_inv_case_
   | _; _ ⊢ fold<_> _ : _ => tac type_inv_fold
   | _; _ ⊢ unfold<_> _ : _ => tac type_inv_unfold
+  | _; _ ⊢ mux _ _ _ : _ => tac type_inv_mux
+  | _; _ ⊢ tape _ : _ => tac type_inv_tape
   | _; _ ⊢ [_] : _ => tac type_inv_boxedlit
   | _; _ ⊢ [inj@_<_> _] : _ => tac type_inv_boxedinj
   | _; _ ⊢ _ * _ : _ => apply type_inv_prod in H; elim H
